case_study/RiscvPmp/BlockVer/Spec.v
@@ -108,7 +108,7 @@ Module RiscvPmpBlockVerifSpec <: Specification RiscvPmpBase RiscvPmpSignature Ri
   Notation asn_pmp_addr_access l m := (asn.chunk (chunk_user pmp_addr_access [l; m])).
   Notation asn_pmp_access addr width es m p := (asn.formula (formula_user pmp_access [addr;width;es;m;p])).
   Notation asn_mmio_pred bytes := (asn.chunk (chunk_user (mmio_trace bytes) [env])).
-  Notation asn_mmio_checked_write bytes a w := (asn.chunk (chunk_user (mmio_checked_write bytes) [a; w])).
+  Notation asn_mmio_checked_write bytes a w s s' := (asn.chunk (chunk_user (mmio_checked_write bytes) [a; w; s; s'])).
 
   Definition term_eqb {Σ} (e1 e2 : Term Σ ty_regno) : Term Σ ty.bool :=
     term_binop (bop.relop bop.eq) e1 e2.
@@ -221,9 +221,9 @@ Module RiscvPmpBlockVerifSpec <: Specification RiscvPmpBase RiscvPmpSignature Ri
   Local Notation asn_cur_privilege val := (asn.chunk (chunk_ptsreg cur_privilege val)).
   Local Notation asn_bool t := (asn.formula (formula_bool t)).
   Local Notation asn_in_mmio n l := (asn.formula (formula_user (in_mmio n) [l])).
-  Local Notation asn_mmio_state_pred bytes s w := (asn.chunk (chunk_user (mmio_state bytes) [s; w])).
+  Local Notation asn_mmio_state_pred bytes s := (asn.chunk (chunk_user (mmio_state bytes) [s])).
   Local Notation asn_mmio_trace_pred bytes := (asn.chunk (chunk_user (mmio_trace bytes) [env])).
-  Local Notation asn_mmio_checked_write bytes a w := (asn.chunk (chunk_user (mmio_checked_write bytes) [a; w])).
+  Local Notation asn_mmio_checked_write bytes a w s s' := (asn.chunk (chunk_user (mmio_checked_write bytes) [a; w; s; s'])).
   Import bv.notations.
 
   Definition sep_contract_rX : SepContractFun rX :=
@@ -281,24 +281,24 @@ Module RiscvPmpBlockVerifSpec <: Specification RiscvPmpBase RiscvPmpSignature Ri
          asn.match_bool (term_var "inv") (term_var "paddr" ↦ᵣ[ bytes ] term_var "w") (term_var "paddr" ↦ₘ[ bytes ] term_var "w");
     |}.
 
-
   Definition sep_contract_checked_mem_write {bytes} {H: restrict_bytes bytes} : SepContractFun (@checked_mem_write bytes H) :=
-    {| sep_contract_logic_variables := ["inv" :: ty.bool; "paddr" :: ty_xlenbits; "data" :: ty_bytes bytes; "iostate" :: ty.bool];
+    {| sep_contract_logic_variables := ["write_mmio" :: ty.bool; "paddr" :: ty_xlenbits; "data" :: ty_bytes bytes; "iostate_old" :: ty.bool; "iostate_new" :: ty.bool];
       sep_contract_localstore      := [term_var "paddr"; term_var "data"];
       sep_contract_precondition    :=
-        asn.match_bool (term_var "inv")
+        asn.match_bool (term_var "write_mmio")
           (asn_in_mmio bytes (term_var "paddr") ∗
            term_binop bop.plus (term_unsigned (term_var "paddr")) (term_val ty.int (Z.of_nat bytes)) < (term_val ty.int (Z.of_N (bv.exp2 xlenbits))) ∗
-           asn_mmio_state_pred bytes (term_var "iostate") (term_var "data") ∗
-           asn_mmio_trace_pred bytes ∗
-           asn_mmio_checked_write bytes (term_var "paddr") (term_var "data"))
+           (asn_mmio_trace_pred bytes) ∗
+           (asn_mmio_state_pred bytes (term_var "iostate_old")) ∗
+           (asn_mmio_checked_write bytes (term_var "paddr") (term_var "data") (term_var "iostate_old") (term_var "iostate_new"))
+          )
           (∃ "w", term_var "paddr" ↦ₘ[ bytes ] term_var "w" ∗
            (term_val ty.int (Z.of_N minAddr) <= term_unsigned (term_var "paddr"))%asn ∗
            (term_binop bop.plus (term_unsigned (term_var "paddr")) (term_val ty.int (Z.of_nat bytes))) <= term_val ty.int (Z.of_N maxAddr));
       sep_contract_result          := "result_checked_mem_write";
       sep_contract_postcondition   :=
         term_var "result_checked_mem_write" = term_union (memory_op_result 1) KMemValue (term_val ty_byte [bv 1]) ∗
-        asn.match_bool (term_var "inv") (asn_mmio_state_pred bytes (term_var "iostate") (term_var "data") ∗ asn_mmio_trace_pred bytes) (term_var "paddr" ↦ₘ[ bytes ] term_var "data");
+        asn.match_bool (term_var "write_mmio") ⊤ (term_var "paddr" ↦ₘ[ bytes ] term_var "data");
     |}.
 
   Definition sep_contract_pmpCheck {bytes : nat} {H : restrict_bytes bytes} : SepContractFun (@pmpCheck bytes H) :=
@@ -334,14 +334,17 @@ Module RiscvPmpBlockVerifSpec <: Specification RiscvPmpBase RiscvPmpSignature Ri
     |}.
 
   Definition sep_contract_pmp_mem_write {bytes} {H: restrict_bytes bytes} : SepContractFun (@pmp_mem_write bytes H) :=
-    {| sep_contract_logic_variables := ["inv" :: ty.bool; "paddr" :: ty_xlenbits; "data" :: ty_bytes bytes; "typ" :: ty_access_type; "m" :: ty_privilege; "entries" :: ty.list ty_pmpentry];
+    {| sep_contract_logic_variables := ["write_mmio" :: ty.bool; "paddr" :: ty_xlenbits; "data" :: ty_bytes bytes; "typ" :: ty_access_type; "m" :: ty_privilege; "entries" :: ty.list ty_pmpentry; "iostate_old" :: ty.bool; "iostate_new" :: ty.bool];
       sep_contract_localstore      := [term_var "paddr"; term_var "data"; term_var "typ"; term_var "m"];
       sep_contract_precondition    :=
-        asn.match_bool (term_var "inv")
-          (asn_in_mmio bytes (term_var "paddr") ∗
-           term_binop bop.plus (term_unsigned (term_var "paddr")) (term_val ty.int (Z.of_nat bytes)) < (term_val ty.int (Z.of_N (bv.exp2 xlenbits))) ∗
-           asn_mmio_trace_pred bytes ∗
-           asn_mmio_checked_write bytes (term_var "paddr") (term_var "data"))
+        asn.match_bool (term_var "write_mmio")
+          (
+           (asn_in_mmio bytes (term_var "paddr")) ∗
+           (term_binop bop.plus (term_unsigned (term_var "paddr")) (term_val ty.int (Z.of_nat bytes)) < (term_val ty.int (Z.of_N (bv.exp2 xlenbits)))) ∗
+           (asn_mmio_trace_pred bytes) ∗
+           (asn_mmio_state_pred bytes (term_var "iostate_old")) ∗
+           (asn_mmio_checked_write bytes (term_var "paddr") (term_var "data") (term_var "iostate_old") (term_var "iostate_new"))
+          )
           (∃ "w", term_var "paddr" ↦ₘ[ bytes ] term_var "w" ∗
            (term_val ty.int (Z.of_N minAddr) <= term_unsigned (term_var "paddr"))%asn ∗
            (term_binop bop.plus (term_unsigned (term_var "paddr")) (term_val ty.int (Z.of_nat bytes))) <= term_val ty.int (Z.of_N maxAddr)) ∗
@@ -352,10 +355,11 @@ Module RiscvPmpBlockVerifSpec <: Specification RiscvPmpBase RiscvPmpSignature Ri
       sep_contract_result          := "result_mem_write";
       sep_contract_postcondition   :=
         term_var "result_mem_write" = term_union (memory_op_result 1) KMemValue (term_val ty_byte [bv 1]) ∗
-        asn.match_bool (term_var "inv") (asn_mmio_trace_pred bytes) (term_var "paddr" ↦ₘ[ bytes ] term_var "data") ∗
+        asn.match_bool (term_var "write_mmio") ⊤ (term_var "paddr" ↦ₘ[ bytes ] term_var "data") ∗
         asn_cur_privilege (term_var "m") ∗
         asn_pmp_entries (term_var "entries");
     |}.
+
 
   Definition sep_contract_mem_read {bytes} {H : restrict_bytes bytes} : SepContractFun (@mem_read bytes H) :=
     {| sep_contract_logic_variables := ["inv" :: ty.bool; "typ" :: ty_access_type; "paddr" :: ty_xlenbits; "entries" :: ty.list ty_pmpentry; "w" :: ty_bytes bytes];
@@ -375,16 +379,20 @@ Module RiscvPmpBlockVerifSpec <: Specification RiscvPmpBase RiscvPmpSignature Ri
           asn_pmp_entries (term_var "entries");
     |}.
 
+
   (* Access type `Write` needed here, as `mem_write_value` calls `pmp_mem_write` with this access type*)
   Definition sep_contract_mem_write_value {bytes} {H: restrict_bytes bytes} : SepContractFun (@mem_write_value bytes H) :=
-    {| sep_contract_logic_variables := ["inv" :: ty.bool; "paddr" :: ty_xlenbits; "data" :: ty_bytes bytes; "entries" :: ty.list ty_pmpentry];
+    {| sep_contract_logic_variables := ["write_mmio" :: ty.bool; "paddr" :: ty_xlenbits; "data" :: ty_bytes bytes; "entries" :: ty.list ty_pmpentry; "iostate_old" :: ty.bool; "iostate_new" :: ty.bool];
       sep_contract_localstore      := [term_var "paddr"; term_var "data"];
       sep_contract_precondition    :=
-        asn.match_bool (term_var "inv")
-          (asn_in_mmio bytes (term_var "paddr") ∗
-           term_binop bop.plus (term_unsigned (term_var "paddr")) (term_val ty.int (Z.of_nat bytes)) < (term_val ty.int (Z.of_N (bv.exp2 xlenbits))) ∗
-           asn_mmio_trace_pred bytes ∗
-           asn_mmio_checked_write bytes (term_var "paddr") (term_var "data"))
+        asn.match_bool (term_var "write_mmio")
+          (
+            (asn_in_mmio bytes (term_var "paddr")) ∗
+              (term_binop bop.plus (term_unsigned (term_var "paddr")) (term_val ty.int (Z.of_nat bytes)) < (term_val ty.int (Z.of_N (bv.exp2 xlenbits)))) ∗
+              (asn_mmio_state_pred bytes (term_var "iostate_old")) ∗
+              (asn_mmio_trace_pred bytes) ∗
+              (asn_mmio_checked_write bytes (term_var "paddr") (term_var "data") (term_var "iostate_old") (term_var "iostate_new"))
+          )
           (∃ "w", term_var "paddr" ↦ₘ[ bytes ] term_var "w" ∗
            (term_val ty.int (Z.of_N minAddr) <= term_unsigned (term_var "paddr"))%asn ∗
            (term_binop bop.plus (term_unsigned (term_var "paddr")) (term_val ty.int (Z.of_nat bytes))) <= term_val ty.int (Z.of_N maxAddr)) ∗
@@ -394,7 +402,7 @@ Module RiscvPmpBlockVerifSpec <: Specification RiscvPmpBase RiscvPmpSignature Ri
       sep_contract_result          := "result_mem_write";
       sep_contract_postcondition   :=
         term_var "result_mem_write" = term_union (memory_op_result 1) KMemValue (term_val ty_byte [bv 1]) ∗
-        asn.match_bool (term_var "inv") (asn_mmio_trace_pred bytes) (term_var "paddr" ↦ₘ[ bytes ] term_var "data") ∗
+        asn.match_bool (term_var "write_mmio") (asn_mmio_trace_pred bytes) (term_var "paddr" ↦ₘ[ bytes ] term_var "data") ∗
         asn_cur_privilege (term_val ty_privilege Machine) ∗
         asn_pmp_entries (term_var "entries");
     |}.
@@ -489,19 +497,19 @@ Module RiscvPmpBlockVerifSpec <: Specification RiscvPmpBase RiscvPmpSignature Ri
   (* NOTE: for now no resources in `POST`; add those once we need to reinstate local state *)
   (* NOTE: if overflow is important, a no-overflow statement can be added to the `asn_mmio_checked_write` resource *)
   Definition sep_contract_mmio_write (bytes : nat) {H: restrict_bytes bytes} : SepContractFunX (mmio_write H) :=
-    {| sep_contract_logic_variables := ["paddr" :: ty_xlenbits; "data" :: ty_bytes bytes; "iostate" :: ty.bool ; "newiostate" :: ty.bool ];
+    {| sep_contract_logic_variables := ["paddr" :: ty_xlenbits; "data" :: ty_bytes bytes; "iostate_old" :: ty.bool; "iostate_new" :: ty.bool ];
         sep_contract_localstore      := [term_var "paddr"; term_var "data"];
         sep_contract_precondition    :=
            asn_in_mmio bytes (term_var "paddr") ∗
-           asn_mmio_state_pred bytes (term_var "iostate") ∗
-           asn_mmio_checked_write bytes (term_var "paddr") (term_var "iostate") (term_var "data") (term_var "newiostate");
+           asn_mmio_trace_pred bytes ∗
+           asn_mmio_state_pred bytes (term_var "iostate_old") ∗
+           asn_mmio_checked_write bytes (term_var "paddr") (term_var "data") (term_var "iostate_old") (term_var "iostate_new");
       sep_contract_result          := "result_write_mmio";
       sep_contract_postcondition   :=
-                                       term_var "result_write_mmio" = term_val ty.bool true ∗
+        term_var "result_write_mmio" = term_val ty.bool true ∗
                                        asn_in_mmio bytes (term_var "paddr") ∗
-                                       asn_mmio_state_pred bytes (term_var "iostate") (term_var "data") ∗
-                                       asn_mmio_checked_write bytes (term_var "paddr") (term_var "data"); 
-
+                                       asn_mmio_trace_pred bytes ∗
+                                       asn_mmio_state_pred bytes (term_var "iostate_new");
     |}.
 
   Definition sep_contract_decode    : SepContractFunX decode :=
@@ -585,23 +593,23 @@ Module RiscvPmpBlockVerifSpec <: Specification RiscvPmpBase RiscvPmpSignature Ri
   Proof. destruct widthh; now compute. Qed.
   Local Hint Resolve wordwidth_upper_bound : typeclass_instances.
 
-  Import TermNotations.
+  Import
+    TermNotations.
   Definition lemma_close_mmio_write (immm : bv 12) (widthh : WordWidth) : SepLemma (close_mmio_write immm widthh) :=
-    {| lemma_logic_variables := ["paddr" :: ty_xlenbits; "r" :: ty_regno; "w" :: ty_word; "s" :: ty.bool ];
+    {| lemma_logic_variables := ["paddr" :: ty_xlenbits; "r" :: ty_regno; "w" :: ty_word; "iostate_old" :: ty.bool ];
       lemma_patterns        := [term_var "paddr"; term_var "r"];
       lemma_precondition    :=
         ((term_val ty_xlenbits RiscvPmpIrisInstance.write_addr) = (term_var "paddr" +ᵇ term_sext (term_val (ty.bvec 12) immm))) ∗
           (term_var "r") ↦ᵣ (term_var "w") ∗
-          (asn.chunk (chunk_user (mmio_state bytes_per_word) [term_var "s"])) ∗
           (* depending on the protocol state, the value should be either even or odd *)
-          asn.match_bool s
-          (term_unop (uop.bvtake 1) (term_var "w") = term_val (ty.bvec 1) (bv.of_N 1))
-          (term_unop (uop.bvtake 1) (term_var "w") = term_val (ty.bvec 1) (bv.of_N 0));
+          asn.match_bool (term_var "iostate_old")
+            (term_unop (uop.bvtake 1) (term_var "w") = term_val (ty.bvec 1) (bv.one))
+            (term_unop (uop.bvtake 1) (term_var "w") = term_val (ty.bvec 1) (bv.zero));
       lemma_postcondition   :=
-        (asn.chunk (chunk_user (mmio_state bytes_per_word) [term_var "s"])) ∗
-        asn_mmio_checked_write (map_wordwidth widthh) s (term_var "paddr" +ᵇ term_sext (term_val (ty.bvec 12) immm)) (term_truncate (map_wordwidth widthh * byte) (term_var "w")) (term_unop uop.not s) ∗
-      ( term_var "r") ↦ᵣ (term_var "w");
+        (term_var "r") ↦ᵣ (term_var "w") ∗
+        asn_mmio_checked_write (map_wordwidth widthh) (term_var "paddr" +ᵇ term_sext (term_val (ty.bvec 12) immm)) (term_truncate (map_wordwidth widthh * byte) (term_var "w")) (term_var "iostate_old") (term_unop uop.not (term_var "iostate_old"));
     |}.
+
 
    Definition LEnv : LemmaEnv :=
      fun Δ l =>
@@ -614,7 +622,7 @@ Module RiscvPmpBlockVerifSpec <: Specification RiscvPmpBase RiscvPmpSignature Ri
        | close_pmp_entries            => lemma_close_pmp_entries
        | extract_pmp_ptsto bytes      => lemma_extract_pmp_ptsto bytes
        | return_pmp_ptsto bytes       => lemma_return_pmp_ptsto bytes
-       | close_mmio_write immm widthh => lemma_close_mmio_write immm widthh 
+       | close_mmio_write immm widthh => lemma_close_mmio_write immm widthh
       end.
 End RiscvPmpBlockVerifSpec.
 
@@ -691,14 +699,9 @@ Module RiscvPmpSpecVerif.
   Lemma valid_pmp_mem_read {bytes} {H : restrict_bytes bytes} : ValidContract (@pmp_mem_read bytes H).
   Proof. destruct H; now vm_compute. Qed.
 
-  (* fdu: debug *)
-  Import SymProp.notations.
-  Set Printing Depth 200.
- 
-  Lemma valid_pmp_mem_write {bytes} {H : restrict_bytes bytes} : ValidContract (@pmp_mem_write bytes H).
-  Proof.
-    destruct H; now vm_compute. Qed.
-  Admitted.
+  Lemma valid_pmp_mem_write {bytes} {H : restrict_bytes bytes} : ValidContractDebug (@pmp_mem_write bytes H).
+  Proof. destruct H; vm_compute; (constructor; simpl; intros; exists v3; exists v4; done).
+  Qed.
 
   Import Bitvector.bv.notations.
 
@@ -710,36 +713,38 @@ Module RiscvPmpSpecVerif.
   Qed.
 
   Lemma valid_pmpCheck {bytes : nat} {H : restrict_bytes bytes} : ValidContractWithFuelDebug 4 (@pmpCheck bytes H).
-  Proof.
-  (*   destruct H; apply verification_condition_with_erasure_sound; vm_compute; *)
-  (*     constructor; cbn; *)
-  (*     repeat (intros; split; intros); *)
-  (*     repeat match goal with *)
-  (*       | H: (?b1 || ?b2)%bool = true |- _ => *)
-  (*           apply Bool.orb_true_iff in H *)
-  (*       | H: ?P /\ ?Q |- _ => *)
-  (*           destruct H *)
-  (*       | H: ?P \/ ?Q |- _ => *)
-  (*           destruct H as [H|H] *)
-  (*       | H: negb ?b = true |- _ => *)
-  (*           apply Bool.negb_true_iff in H; *)
-  (*           subst *)
-  (*       | H1: ?a <=ᵘ ?b, H2: ?b <ᵘ ?a |- False => *)
-  (*           unfold bv.ult, bv.ule in *; apply N.le_ngt in H1; apply (H1 H2) *)
-  (*       end; *)
-  (*     subst; *)
-  (*     unfold Pmp_check_perms, decide_pmp_check_perms, pmp_check_RWX in *; *)
-  (*     simpl in *; *)
-  (*     try discriminate; *)
-  (*     try bv_solve_Ltac.solveBvManual. *)
-  (* Qed. *)
+(*   Proof. *)
+(*     destruct H; apply verification_condition_with_erasure_sound; vm_compute;
+      constructor; cbn;
+      repeat (intros; split; intros);
+      repeat match goal with
+        | H: (?b1 || ?b2)%bool = true |- _ =>
+            apply Bool.orb_true_iff in H
+        | H: ?P /\ ?Q |- _ =>
+            destruct H
+        | H: ?P \/ ?Q |- _ =>
+            destruct H as [H|H]
+        | H: negb ?b = true |- _ =>
+            apply Bool.negb_true_iff in H;
+            subst
+        | H1: ?a <=ᵘ ?b, H2: ?b <ᵘ ?a |- False =>
+            unfold bv.ult, bv.ule in *; apply N.le_ngt in H1; apply (H1 H2)
+        end;
+      subst;
+      unfold Pmp_check_perms, decide_pmp_check_perms, pmp_check_RWX in *;
+      simpl in *;
+      try discriminate;
+      try bv_solve_Ltac.solveBvManual.
+  Qed. *)
 Admitted.
 
   Lemma valid_mem_read {bytes} {H : restrict_bytes bytes} : ValidContract (@mem_read bytes H).
   Proof. now destruct H. Qed.
 
-  Lemma valid_mem_write_value {bytes} {H : restrict_bytes bytes} : ValidContract (@mem_write_value bytes H).
-  Proof. now destruct H. Qed.
+  Lemma valid_mem_write_value {bytes} {H : restrict_bytes bytes} : ValidContractDebug (@mem_write_value bytes H).
+  Proof.
+    destruct H; vm_compute; constructor; intros; simpl; eauto.
+  Qed.
 
   Lemma valid_contract_within_phys_mem : ValidContractDebug within_phys_mem.
   Proof. symbolic_simpl. intros. Lia.lia. Qed.
@@ -763,6 +768,10 @@ Admitted.
       RiscvPmpBlockVerifSpec.CEnv f = Some c ->
       ValidContractWithFuelDebug fuel f ->
       Symbolic.ValidContractWithFuel fuel c (FunDef f).
+
+
+
+
   Proof.
     intros ? ? fuel f c Hcenv Hvc.
     unfold ValidContractWithFuelDebug in Hvc.
@@ -793,10 +802,10 @@ Admitted.
     - refine (valid_contract _ H valid_checked_mem_read).
     - refine (valid_contract _ H valid_checked_mem_write).
     - refine (valid_contract _ H valid_pmp_mem_read).
-    - refine (valid_contract _ H valid_pmp_mem_write).
+    - refine (valid_contract_debug _ H valid_pmp_mem_write).
     - refine (valid_contract_with_fuel_debug _ _ H valid_pmpCheck).
     - refine (valid_contract_debug _ H valid_pmpMatchAddr).
-    - refine (valid_contract _ H valid_mem_write_value).
+    - refine (valid_contract_debug _ H valid_mem_write_value).
     - refine (valid_contract _ H valid_execute_fetch).
     - refine (valid_contract_debug _ H valid_contract_execute_EBREAK).
   Qed.
@@ -833,7 +842,7 @@ Module RiscvPmpIrisInstanceWithContracts.
   Proof.
       intros Γ es δ ι Heq. cbn. destruct_syminstance ι.
       iIntros "H". cbn in *. iApply semTWP_foreign.
-      iIntros (? ?) "(Hregs & % & Hmem & %Hmap & Htr & Hst)".
+      iIntros (? ?) "(Hregs & % & Hmem & %Hmap & Htr)".
       iMod (fupd_mask_subseteq empty) as "Hclose"; auto. iModIntro.
       iIntros (res ? ? Hf). rewrite Heq in Hf. cbn in Hf. inversion Hf; subst.
       iMod "Hclose" as "_". destruct inv.
@@ -842,13 +851,13 @@ Module RiscvPmpIrisInstanceWithContracts.
         iInv "H" as "Hptsto" "Hclose_ptsto".
         iDestruct (bi.later_mono _ _ (RiscvPmpModel2.fun_read_ram_works Hmap) with "[$Hptsto $Hmem]") as "#>%eq_fun_read_ram".
         iMod ("Hclose_ptsto" with "Hptsto") as "_". iModIntro.
-        iFrame "Hregs Hmem Hst Htr". iSplitR; first auto.
+        iFrame "Hregs Hmem Htr". iSplitR; first auto.
         iApply semTWP_val. iModIntro.
         now iFrame "H".
       - (* old case *)
         iModIntro.
         iPoseProof (RiscvPmpModel2.fun_read_ram_works Hmap with "[$H $Hmem]") as "%eq_fun_read_ram".
-        iPoseProof (RiscvPmpModel2.mem_inv_not_modified $! Hmap with "Hmem Hst Htr") as "Hmem".
+        iPoseProof (RiscvPmpModel2.mem_inv_not_modified $! Hmap with "Hmem Htr") as "Hmem".
         iFrame "Hregs Hmem". iApply semTWP_val. now iFrame "H".
   Qed.
 
@@ -857,64 +866,51 @@ Module RiscvPmpIrisInstanceWithContracts.
   Proof.
     intros Γ es δ ι Heq. destruct_syminstance ι. cbn in *.
     iIntros "[%w H]". iApply semTWP_foreign.
-    iIntros (? ?) "(Hregs & % & Hmem & %Hmap & Htr & Hst)".
+    iIntros (? ?) "(Hregs & % & Hmem & %Hmap & Htr)".
     iMod (fupd_mask_subseteq empty) as "Hclose"; auto. iModIntro.
     iIntros (res ? ? Hf). rewrite Heq in Hf. cbn in Hf. inversion Hf; subst.
     iMod "Hclose" as "_".
-    iMod (RiscvPmpModel2.fun_write_ram_works with "[$H $Hmem $Htr $Hst]") as "[$ H]"; auto.
+    iMod (RiscvPmpModel2.fun_write_ram_works with "[$H $Hmem $Htr]") as "[$ H]"; auto.
     rewrite semTWP_val. now iFrame "Hregs H".
  Qed.
-
-  (* Important sanity condition on mmio predicates - NOTE: could be in typeclass, together with the condition that reads are either all accepted, or none of them are *)
-  Lemma mmio_pred_cons {bytes : nat} t e : event_pred bytes e → mmio_trace_pred bytes t → mmio_trace_pred bytes (cons e t).
-  Proof.
-    unfold mmio_trace_pred. intros. destruct H0; auto.
-  Qed.
 
   Lemma mmio_write_sound `{!sailGS Σ} `(H: restrict_bytes bytes) :
     TValidContractForeign (@RiscvPmpBlockVerifSpec.sep_contract_mmio_write _ H) (mmio_write H).
   Proof.
     intros Γ es δ ι Heq. destruct_syminstance ι. cbn in *.
-    iIntros "([%Hmmio _] & [%e %Hstate] & #Hinv & [-> [%v ->]])". iApply semTWP_foreign.
-    iIntros (? ?) "[Hregs [% (Hmem & %Hmap & Htra & Hstf)]]".
-    iInv "Hinv" as "Hpred" "Hclose".
-    iDestruct "Hpred" as (s t) "(>Htrf & >Hsta & >%Hpred)".
+    iIntros "([%Hmmio _] & #Hinv & Hstf & (-> & %Hstate))".
+    iApply semTWP_foreign.
+    iIntros (? ?) "[Hregs [%a (Hmem & %Hmap & Htra)]]".
+    iInv "Hinv" as (s t) "(>Htrf & >Hsta & >%Hpred)" "Hclose".
     iDestruct (trace.trace_full_frag_eq with "Htra Htrf") as "%Heqt". subst.
     iDestruct (trace.iost_full_frag_eq with "Hsta Hstf") as "%Heqs". subst.
     iMod (trace.trace_update _ _ (cons _ _) with "[$Htra $Htrf]") as "[Htra Htrf]".
     iMod (trace.state_update _ _ _ with "[$Hsta $Hstf]") as "[Hsta Hstf]".
     iMod ("Hclose" with "[Htrf Hsta]") as "_".
     {(* Instantiate evars *)
-      iNext. iExists _, _. iFrame. iPureIntro.
-      apply mmio_pred_cons; [|eauto]. unfold event_pred. exists v. eauto.
-    }
-    iMod (fupd_mask_subseteq empty) as "Hclose"; first set_solver.
-    iModIntro.
+      iExists _. iExists _. iNext. iFrame.
+      iPureIntro. econstructor; eauto.
+      }
+    iMod (fupd_mask_subseteq empty) as "Hclose"; auto. iModIntro.
     iIntros (res ? ? Hf). rewrite Heq in Hf. cbn in Hf. inversion Hf; subst.
-    rewrite semTWP_val.
+    iMod "Hclose" as "_". rewrite semTWP_val.
     destruct bytes; first contradiction.
-    iFrame "Hinv Hregs Hmem Htra Hstf".
-    iMod "Hclose" as "_".
-    iModIntro. iSplitL; auto.
-    iModIntro. iSplitR; auto.
-    iSplitR; auto.
-    iSplitR.
-    - unfold interp_mmio_state_pred, mmio_state_pred. iPureIntro. exists e. apply Hstate.
-    - unfold interp_mmio_checked_write. iPureIntro. split; auto. exists v. auto.
+    unfold mem_inv, fun_write_mmio; cbn.
+    iFrame "Hregs Hmem Htra Hstf".
+    repeat iSplitL; auto.
   Qed.
-
 
   Lemma decode_sound `{sailGS Σ} :
     TValidContractForeign RiscvPmpBlockVerifSpec.sep_contract_decode RiscvPmpProgram.decode.
   Proof.
     intros Γ es δ ι Heq. destruct_syminstance ι. cbn in *.
     iIntros "%Hdecode". iApply semTWP_foreign.
-    iIntros (? ?) "[Hregs [% (Hmem & %Hmap & Htr & Hst)]]".
+    iIntros (? ?) "[Hregs [% (Hmem & %Hmap & Htr)]]".
     iMod (fupd_mask_subseteq empty) as "Hclose"; auto. iModIntro.
     iIntros (? ? ? Hf). iMod "Hclose" as "_".
     rewrite Heq in Hf. cbn in Hf. inversion Hf; subst.
     destruct (pure_decode _); inversion Hdecode.
-    iPoseProof (RiscvPmpModel2.mem_inv_not_modified $! Hmap with "Hmem Hst Htr") as "Hmem".
+    iPoseProof (RiscvPmpModel2.mem_inv_not_modified $! Hmap with "Hmem Htr") as "Hmem".
     rewrite semTWP_val. now iFrame "Hregs Hmem".
   Qed.
 
@@ -990,17 +986,24 @@ Module RiscvPmpIrisInstanceWithContracts.
     now iFrame.
   Qed.
 
+
   Lemma close_mmio_write_sound `{sailGS Σ} (imm : bv 12) (width : WordWidth) :
     ValidLemma (RiscvPmpBlockVerifSpec.lemma_close_mmio_write imm width ).
   Proof.
     intros ι; destruct_syminstance ι; cbn.
-    iIntros "([<- _] & Hmmio & _)".
-    unfold interp_mmio_checked_write.
+    iIntros "([<- _] & Hmmio & Hcond)".
     iFrame.
-    iPureIntro.
-    split; auto.
-    eexists. destruct width; reflexivity.
-  Qed.
+    unfold interp_mmio_checked_write. cbn in *.
+    destruct iostate_old; iDestruct "Hcond" as "[Hcond _]"; cbn; subst; iSplitR; auto;
+      unfold inst; unfold inst_term; unfold RiscvPmpBlockVerifSpec.map_wordwidth; cbn;
+      iDestruct "Hcond" as "%Hcond"; iPureIntro; simpl in *.
+      - assert (HH: width = WORD).  admit. subst. cbn.
+        eapply IOW_even_odd; simpl in *; try lia; eauto.
+        erewrite Hcond. auto.
+      - assert (HH: width = WORD). admit. subst. cbn.
+        eapply IOW_odd_even; simpl in *; try lia; eauto.
+        erewrite Hcond. auto.
+ Admitted.
 
   Lemma lemSemBlockVerif `{sailGS Σ} : LemmaSem.
   Proof.
